\chapter{Trigonometric Identities}

\section{The Unit Circle}
There are some values of $\sin{\theta}$ and $\cos{\theta}$ that will be 
useful to know off the top of your head. The Unit Circle will help you in this 
memorization process (see figure \ref{fig:unit_cicle_blank}). When a circle of 
radius 1 is centered at the origin, the Cartesian coordinates of any point on 
the circle correspond to the values of cosine and sine of the angle above 
the horizontal (how far you've rotated from the positive $x$-axis). 

\begin{figure}[htbp]
    \centering
    \begin{tikzpicture}
        \draw[-latex, thick] (-3, 0) -- (3, 0) node[right] {$x$};
        \draw[-latex, thick] (0, -3) -- (0, 3) node[above] {$y$};
        \draw[blue, thick] (0,0) circle (2);
        \draw[blue, dashed] (0,0) -- (1, 1.732);
        \draw[blue, fill=blue] (1, 1.732) circle (0.05);
        \node[blue] at (1.8, 2) {$(\cos{\theta}$, $\sin{\theta})$};
        \draw[black, dashed] (0,0) -- (1.414, -1.414);
        \node[] at (1.8, -1.8) {$r=1$};
    \end{tikzpicture}
    \caption{The Unit Circle is a circle with radius 1 centered at the origin}
    \label{fig:unit_cicle_blank}
\end{figure}

Let's take a closer look at a triangle in the first quadrant to see why this 
is true. Imagine some point on the circle, $(x_o, y_o)$. Drawing a line from 
that point back to the origin creates an angle $\theta$ between the imaginary 
line and the positive $x$-axis (see figure \ref{fig:unit_cicle_zoom}). 
Extending an imaginary vertical down to $(x_o, 0)$, then an imaginary 
horizontal from $(x_o, 0)$ to the origin, creates a right triangle. What can we 
say about the legs of the triangle?

\begin{figure}[htbp]
    \centering
    \begin{tikzpicture}
        \draw[-latex, thick] (0, 0) -- (4, 0) node[right] {$x$};
        \draw[-latex, thick] (0, 0) -- (0, 4) node[above] {$y$};
        \draw[blue, thick] (3,0) arc [start angle = 0, end angle = 90, 
        x radius = 3, y radius = 3];
        \draw[black, dashed] (0,0) -- (1.5, 2.598);
        \draw[black, very thin] (0.5, 0) arc [start angle = 0, end angle = 60, 
        x radius = 0.5, y radius = 0.5];
        \node[] at (1.7, 3) {$(x_o$, $y_o)$};
        \node[] at (0.7, 0.3) {$\theta$};
        \draw[red, thick, dashed] (0,0) -- (1.5, 0) -- (1.5, 2.598);
        \draw[decorate, decoration=brace] (1.6, 2.598) -- (1.6, 0) node[midway, 
        xshift = 0.3cm] {$y_o$};
        \draw[decorate, decoration=brace] (1.5, -0.1) -- (0, -0.1) node[midway, 
        yshift = -0.3cm] {$x_o$};
    \end{tikzpicture}
    \caption{Drawing a line from any point on the circle to the origin creates 
    an angle with the horizontal}
    \label{fig:unit_cicle_zoom}
\end{figure}

Recall SOH-CAH-TOA from a previous chapter. This acronym tells us that, for a 
right triangle, the sine of an angle is given by the ratio of the length of the
leg opposite the angle to the hypotenuse. In our case, then, $\sin{\theta} = 
\frac{y_o}{1} = y_o$. [Remember: We are dealing with the Unit Circle, which has
a radius of one. Examining figure \ref{fig:unit_cicle_zoom} shows you that the 
hypotenuse of the imaginary triangle is the same as the circle's radius.] This 
means that the $y$-coordinate of any point on the Unit Circle is the sine of 
the angle of rotation from the horizontal. 

\begin{Exercise}[label = sine]
In a similar manner as we did with $\sin{\theta}$ above, prove the 
$x$-coordinate of any point on the unit circle is equal to $\cos{\theta}$, 
where $\theta$ is the angle of rotation from the horizontal. 
\vspace{20mm}
\end{Exercise}

\begin{Answer}[ref = sine]
We know that for a right triangle, $\cos{\theta} = \frac{\text{adjacent leg}}{
\text{hypotenuse}}$. For a right triangle inscribed in the Unit Circle, the 
adjacent leg is parallel to the $x$-axis and has the same length as the 
$x$-value of the coordinate point on the circle. Additionally, the length of 
the hypotenuse is 1. Therefore, $\cos{\theta} = \frac{x_o}{1} = x_o$. 
\end{Answer}

From these exercises, we can see that each $(x,y)$ coordinate on the circle is equal to $(\cos(\theta), \sin(\theta))$. 

\begin{Exercise}[label = unit_circle1]
Fill in the unit circle with the coordinates for $\theta =$ $0$, $\pi/2$, $\pi$, and $3\pi/2$. Use this to determine:
\begin{enumerate}
\item $\sin{\frac{\pi}{2}}$
\item $\cos{\frac{3\pi}{2}}$
\item $\sin{\pi}$
\item $\cos{-\pi}$

\begin{tikzpicture}
        \draw[thick, -latex] (-2.5, 0) -- (2.5, 0) node[right] {$x$};
        \draw[thick, -latex] (0, -2.5) -- (0, 2.5) node[above] {$y$};
        \draw[blue, thick] (0,0) circle (2);
        
        \draw[blue, fill=blue] (2, 0) circle (0.05);
        \node[blue, font=\tiny] at (2.5, 0.3) {$0$};
        \node[font=\tiny] at (2.7, -0.3) {(\rule{0.3cm}{0.15mm}, \rule{
        0.3cm}{0.15mm})};
        
        \draw[blue, fill=blue] (0, 2) circle (0.05);
        \node[blue, font=\tiny] at (-0.3, 2.2) {$\frac{\pi}{2}$};
        \node[font=\tiny] at (0.5, 2.2) {(\rule{0.3cm}{0.15mm}, \rule{
        0.3cm}{0.15mm})};

        \draw[blue, fill=blue] (-2, 0) circle (0.05);
        \node[blue, font=\tiny] at (-2.5, 0.3) {$\pi$};
        \node[font=\tiny] at (-2.7, -0.3) {(\rule{0.3cm}{0.15mm}, \rule{
        0.3cm}{0.15mm})};

        \draw[blue, fill=blue] (0, -2) circle (0.05);
        \node[blue, font=\tiny] at (-0.3, -2.2) {$\frac{3\pi}{2}$};
        \node[font=\tiny] at (0.5, -2.2) {(\rule{0.3cm}{0.15mm}, \rule{
        0.3cm}{0.15mm})};
    \end{tikzpicture}
\end{enumerate}
\end{Exercise}

\begin{Answer}[ref = unit_circle1]
\begin{enumerate}
\item $\sin{\frac{\pi}{2}} = 1$
\item $\cos{\frac{3\pi}{2}} = 0$
\item $\sin{\pi} = 0$
\item $\cos{-\pi} = -1$ (Negative angles are measured clockwise from the $x$-axis, so $\theta = -\pi$ is at the same angle as $\theta = \pi$.) 
\end{enumerate}

\begin{tikzpicture}
        \draw[thick, -latex] (-2.5, 0) -- (2.5, 0) node[right] {$x$};
        \draw[thick, -latex] (0, -2.5) -- (0, 2.5) node[above] {$y$};
        \draw[blue, thick] (0,0) circle (2);
        
        \draw[blue, fill=blue] (2, 0) circle (0.05);
        \node[blue, font=\tiny] at (2.5, 0.3) {$0$};
        \node[font=\tiny] at (2.7, -0.3) {(1, 0)};
        
        \draw[blue, fill=blue] (0, 2) circle (0.05);
        \node[blue, font=\tiny] at (-0.3, 2.2) {$\frac{\pi}{2}$};
        \node[font=\tiny] at (0.5, 2.2) {(0, 1)};

        \draw[blue, fill=blue] (-2, 0) circle (0.05);
        \node[blue, font=\tiny] at (-2.5, 0.3) {$\pi$};
        \node[font=\tiny] at (-2.7, -0.3) {(-1, 0)};

        \draw[blue, fill=blue] (0, -2) circle (0.05);
        \node[blue, font=\tiny] at (-0.3, -2.2) {$\frac{3\pi}{2}$};
        \node[font=\tiny] at (0.5, -2.2) {(0, -1)};
    \end{tikzpicture}
\end{Answer}

\subsection{Exact Values of Key Angles}
We will examine two triangles. First, a 30-60-90 triangle, then a 45-45-90 triangle. 
As shown in figure \ref{fig:306090}, you can get a 
30-60-90 triangle with hypotenuse 1 by dividing an equilateral triangle in 
half. We will label the horizontal leg of the 30-60-90 triangle A and the 
vertical leg B. 

\begin{figure}[htbp]
    \centering
    \begin{tikzpicture}
        \draw[thick] (-2, 0) -- (2, 0) -- (0, 3.464) -- cycle;
        \draw[dashed] (0,0) -- (0,3.464);
        \draw[decorate, decoration=brace] (-2.1, 0.1) -- (-0.1, 3.564)  node[
        midway, rotate=60, xshift = 0.25cm, yshift = 0.25cm] {hypotenuse = 1};
        \draw[red, decorate, decoration=brace] (0,-0.1) -- (-2, -0.1) node[
        midway, yshift = -0.35cm] {A};
        \draw[blue, decorate, decoration = brace] (0.1, 3.564) -- (0.1, 0)  
        node[midway, xshift=0.35cm] {B};
    \end{tikzpicture}
    \caption{A 30-60-90 triangle is made by vertically bisecting an equilateral
    triangle}
    \label{fig:306090}
\end{figure}

From the figure, we see that the length of A is half that of the hypotenuse, 
which in this case is $\frac{1}{2}$. This means the $\cos{60^{\circ}} = \cos{
\frac{\pi}{3}} = \frac{1}{2}$. To find the length of side B, we can use the 
Pythagorean theorem:
$$B^2 = C^2 - A^2\text{, where C is the hypotenuse}$$
$$B^2 = 1^2 - \left( \frac{1}{2} \right)^2$$
$$B^2 = \frac{3}{4}$$
$$B = \frac{\sqrt{3}}{2}$$

Therefore, $\sin{60^{\circ}} = \sin{\frac{\pi}{3}} = \frac{\sqrt{3}}{2}$. 

\begin{Exercise}[label=unit_circle2]
Use symmetry to complete the blank unit circle below. (Hint: We just showed 
that the $(x,y)$ coordinate for $\frac{\pi}{3}$ is $(1/2, \sqrt{3}/2)$). 

\begin{tikzpicture}
        \draw[thick, -latex] (-2.5, 0) -- (2.5, 0) node[right] {$x$};
        \draw[thick, -latex] (0, -2.5) -- (0, 2.5) node[above] {$y$};
        \draw[blue, thick] (0,0) circle (2);
        \foreach \x/\y/\t in {1.732/1/$\frac{\pi}{6}$, 1/1.732/$\frac{\pi}{3}$,
        -1/1.732/$\frac{2\pi}{3}$, -1.732/1/$\frac{5\pi}{6}$, 
        -1.732/-1/$\frac{7\pi}{6}$, -1/-1.732/$\frac{4\pi}{3}$, 
        1/-1.732/$\frac{5\pi}{3}$, 1.732/-1/$\frac{11\pi}{6}$} {
        \draw[blue, fill=blue] (\x, \y) circle (0.05);
        \node[blue, font=\tiny] at (0.75*\x, 0.75*\y) {\t};
        \node[font=\tiny] at (1.25*\x, 1.25*\y) {(\rule{0.3cm}{0.15mm}, \rule{
        0.3cm}{0.15mm})};
        }
    \end{tikzpicture}
\end{Exercise}

\begin{Answer}[ref = unit_circle2]
\begin{tikzpicture}
        \draw[thick, -latex] (-2.5, 0) -- (2.5, 0) node[right] {$x$};
        \draw[thick, -latex] (0, -2.5) -- (0, 2.5) node[above] {$y$};
        \draw[blue, thick] (0,0) circle (2);
        \foreach \x/\y/\t/\i/\j in {
        1.732/1/$\frac{\pi}{6}$/$\frac{\sqrt{3}}{2}$/$\frac{1}{2}$, 
        1/1.732/$\frac{\pi}{3}$/$\frac{1}{2}$/$\frac{\sqrt{3}}{2}$,
        -1/1.732/$\frac{2\pi}{3}$/$-\frac{1}{2}$/$\frac{\sqrt{3}}{2}$, 
        -1.732/1/$\frac{5\pi}{6}$/$-\frac{\sqrt{3}}{2}$/$\frac{1}{2}$, 
        -1.732/-1/$\frac{7\pi}{6}$/$-\frac{\sqrt{3}}{2}$/$-\frac{1}{2}$, 
        -1/-1.732/$\frac{4\pi}{3}$/$-\frac{1}{2}$/$-\frac{\sqrt{3}}{2}$, 
        1/-1.732/$\frac{5\pi}{3}$/$\frac{1}{2}$/$-\frac{\sqrt{3}}{2}$, 
        1.732/-1/$\frac{11\pi}{6}$/$\frac{\sqrt{3}}{2}$/$-\frac{1}{2}$} {
        \draw[blue, fill=blue] (\x, \y) circle (0.05);
        \node[blue, font=\tiny] at (0.75*\x, 0.75*\y) {\t};
        \node[font=\tiny] at (1.25*\x, 1.25*\y) {(\i, \j)};
        }
    \end{tikzpicture}
\end{Answer}

Now we will look at a 45-45-90 triangle (see figure \ref{fig:454590}), which 
will allow us to complete our Unit Circle. Recall that a 45-45-90 triangle is 
an isosceles triangle in addition to being a right triangle. This means both 
the legs are the same length. Using the Pythagorean theorem, we would say $A = 
B$. We also know that $C = 1$, since our triangle is inscribed in the unit 
circle. Let's find $A$:
$$A^2 + B^2 = C^2$$
$$A^2 + A^2 = 1^2$$
$$2A^2 = 1$$
$$A^2 = \frac{1}{2}$$
$$A = \frac{1}{\sqrt{2}} = \frac{\sqrt{2}}{2}$$

Therefore, each leg has a length of $\sqrt{2}/2$, and the $(x,y)$ coordinates 
for $\theta = 45^{\circ} = \pi/4$ are $(\sqrt{2}/2, \sqrt{2}/2)$. 

\begin{figure}[htbp]
    \centering
    \begin{tikzpicture}
        \draw[thick, -latex] (-0.25, 0) -- (3.5, 0) node[right] {$x$};
        \draw[thick, -latex] (0, -0.25) -- (0, 3.5) node[above] {$y$};
        \draw[blue, thick] (3, 0) arc [start angle = 0, end angle = 90, 
        x radius = 3, y radius = 3];
        \draw[black, dashed] (0,0) -- (2.121, 0) -- (2.121, 2.121) --cycle;
        \draw[blue, decorate, decoration = brace] (0, 0.1) -- (2.121, 2.221) 
        node[rotate = 45, font = \small, midway, yshift = 0.3cm] {$C = 1$};
        \draw[decorate, decoration = brace] (2.121, -0.1) -- (0,-0.1) 
        node[font = \small, midway, yshift = -0.2cm] {$A$};
        \draw[decorate, decoration = brace] (2.221, 2.121) -- (2.221, 0) 
        node[font = \small, midway, xshift = 0.2cm] {$B$};
    \end{tikzpicture}
    \caption{The two legs of a 45-45-90 triangle are the same length}
    \label{fig:454590}
\end{figure}


\begin{Exercise}[label = unit_circle3]
Use symmetry to complete the blank unit circle below.

\begin{tikzpicture}
        \draw[thick, -latex] (-2.5, 0) -- (2.5, 0) node[right] {$x$};
        \draw[thick, -latex] (0, -2.5) -- (0, 2.5) node[above] {$y$};
        \draw[blue, thick] (0,0) circle (2);
        \foreach \x/\y/\t/\i/\j in {
        1.414/1.414/$\frac{\pi}{4}$/$\frac{\sqrt{2}}{2}$/$\frac{\sqrt{2}}{2}$, 
        -1.414/1.414/$\frac{3\pi}{4}$/$-\frac{\sqrt{2}}{2}$/$\frac{\sqrt{2}}{2}$,
        -1.414/-1.414/$\frac{5\pi}{4}$/$-\frac{\sqrt{2}}{2}$/$-\frac{\sqrt{2}}{2}$, 
        1.414/-1.414/$\frac{7\pi}{4}$/$\frac{\sqrt{2}}{2}$/$-\frac{\sqrt{2}}{2}$ } {
        \draw[blue, fill=blue] (\x, \y) circle (0.05);
        \node[blue, font=\tiny] at (0.75*\x, 0.75*\y) {\t};
        \node[font=\tiny] at (1.25*\x, 1.25*\y) {(\rule{0.3cm}{0.15mm}, \rule{
        0.3cm}{0.15mm})};
        }
    \end{tikzpicture}
\end{Exercise}

\begin{Answer}[ref = unit_circle3]
\begin{tikzpicture}
        \draw[thick, -latex] (-2.5, 0) -- (2.5, 0) node[right] {$x$};
        \draw[thick, -latex] (0, -2.5) -- (0, 2.5) node[above] {$y$};
        \draw[blue, thick] (0,0) circle (2);
        \foreach \x/\y/\t/\i/\j in {
        1.414/1.414/$\frac{\pi}{4}$/$\frac{\sqrt{2}}{2}$/$\frac{\sqrt{2}}{2}$, 
        -1.414/1.414/$\frac{3\pi}{4}$/$-\frac{\sqrt{2}}{2}$/$\frac{\sqrt{2}}{2}$,
        -1.414/-1.414/$\frac{5\pi}{4}$/$-\frac{\sqrt{2}}{2}$/$-\frac{\sqrt{2}}{2}$, 
        1.414/-1.414/$\frac{7\pi}{4}$/$\frac{\sqrt{2}}{2}$/$-\frac{\sqrt{2}}{2}$ } {
        \draw[blue, fill=blue] (\x, \y) circle (0.05);
        \node[blue, font=\tiny] at (0.75*\x, 0.75*\y) {\t};
        \node[font=\tiny] at (1.25*\x, 1.25*\y) {(\i, \j)};
        }
    \end{tikzpicture}
\end{Answer}

\begin{Exercise}[label = unit_circle4]
Without a calculator and using only your completed unit circles, determine the 
value requested (angles are given in radians unless otherwise indicated). 
\begin{enumerate}
\item $\cos{\frac{3\pi}{2}}$
\item $\sin{\frac{\pi}{4}}$
\item $\sin{-\frac{\pi}{6}}$
\item $\cos{\frac{4\pi}{3}}$
\item $\sin{\frac{3\pi}{4}}$
\item $\cos{-\frac{\pi}{3}}$
\item $\sin{45^{\circ}}$
\item $\sin{270^{\circ}}$
\item $\sin{-60^{\circ}}$
\item $\sin{150^{\circ}}$
\end{enumerate}
\end{Exercise}

\begin{Answer}[ref = unit_circle4]
\begin{enumerate}
\item $0$
\item $\sqrt{2}/2$
\item $-1/2$
\item $-1/2$
\item $\sqrt{2}/2$
\item $1/2$
\item $\sqrt{2}/2$
\item $-1$
\item $-\sqrt{3}/2$
\item $1/2$
\end{enumerate}
\end{Answer}


\section{Sum and Difference Formulas}
Consider 4 points on the unit circle: $B$ at $(1, 0)$, $Q$ at some angle 
$\beta$, $P$ at some angle $\alpha$, and $A$ at angle $\alpha - \beta$ (see 
figure \ref{fig:difference}). 

\begin{figure}[htbp]
    \centering
    \begin{tikzpicture}
        \draw[-latex, thick] (-4, 0) -- (4, 0) node[right] {$x$};
        \draw[-latex, thick] (0, -0.2) -- (0, 4) node[above] {$y$};
        \draw[blue, thick] (3,0) arc [start angle = 0, end angle = 180, 
        x radius = 3, y radius = 3];
        \draw[thick] (0,0) -- (2.898, 0.776) node[right] {$Q$};
        \draw[thick] (0,0) -- (-1.5, 2.598) node[left, yshift = 0.2cm] {$A$};
        \draw[red, dashed] (2.898, 0.776) -- (-2.121, 2.121);
        \draw[thick] (0,0) -- (-2.121, 2.121) node[left] {$P$};
        \node[] at (3.2, 0.2) {$B$};
        \draw[red, dashed] (-1.5, 2.598) -- (3, 0);
        \draw[thin] (1.5, 0) arc [start angle = 0, end angle = 15, x radius = 
        1.5, y radius = 1.5] node[midway, xshift = 0.2cm] {$\beta$};
        \draw[thin] (1, 0) arc [start angle = 0, end angle = 120, x radius = 1,
        y radius = 1] node[midway, yshift = 0.3cm] {$\alpha - \beta$};
        \draw[thin] (0.5, 0) arc[start angle = 0, end angle = 135, x radius = 
        0.5, y radius = 0.5] node[midway, xshift = 0.1cm, yshift = 0.1cm] 
        {$\alpha$};
    \end{tikzpicture}
    \caption{$\overline{AB} = \overline{PQ}$}
    \label{fig:difference}
\end{figure}

The distance from $P$ to $Q$ is the same as the distance from $A$ to $B$, 
since $\Delta POQ$ is a rotation of $\Delta AOB$. Because this is a Unit 
Circle, $P = (\cos{\alpha}, \sin{\alpha})$, $Q = (\cos{\beta}, \sin{\beta})$, 
and $A = (\cos{\alpha - \beta}, \sin{\alpha - \beta})$. Let's use the distance
formula to find the length of $\overline{PQ}$:
$$\overline{PQ} = \sqrt{\left(\cos{\alpha} - \cos{\beta} \right)^2 + \left( 
\sin{\alpha} - \sin{\beta} \right)^2} =$$
$$\sqrt{\cos^2{\alpha} - 2\cos{\alpha}\cos{\beta} + \cos^2{\beta} + \sin^2{
\alpha} - 2\sin{\alpha}\sin{\beta} + \sin^2{\beta}} = $$
$$\sqrt{\left( \cos^2{\alpha} + \sin^2{\alpha} \right) + \left( \cos^2{\beta} 
+ \sin^2{\beta} \right) - 2\cos{\alpha}\cos{\beta} - 2\sin{\alpha}\sin{\beta}}
$$

Recall that for any angle, $\theta$, $\sin^2{\theta} + \cos^2{\theta} = 1$. 
Substituting this identity, we see that:
$$\overline{PQ} = \sqrt{1 + 1 -2\sin{\alpha}\sin{\beta} - 2\cos{\alpha}\cos{
\beta}} = \sqrt{2 - 2\sin{\alpha}\sin{\beta} - 2\cos{\alpha}\cos{\beta}}$$

Let's leave this simplified equation for $\overline{PQ}$ alone for the moment 
and similarly find $\overline{AB}$:
$$\overline{AB} = \sqrt{\left[ \cos{\left( \alpha - \beta \right)} - 1 \right]^
2 + \left[ \sin{\left( \alpha - \beta \right)} - 0 \right]^2} = $$
$$\sqrt{\cos^2{ \left( \alpha - \beta \right)} - 2\cos{ \left( \alpha - \beta 
\right)} + 1 + \sin^2{ \left( \alpha - \beta \right)}} = $$
$$\sqrt{\cos^2{ \left( \alpha - \beta \right)} + \sin^2{ \left( \alpha - \beta 
\right)} + 1 - 2\cos{ \left( \alpha - \beta \right)}} $$
$$= \sqrt{2 - 2\cos{ \left( \alpha - \beta \right)}} = \overline{AB}$$

Recall that we've established $\overline{AB} = \overline{PQ}$. We can set 
the statements equal to each other:
$$ \sqrt{2 - 2\sin{\alpha}\sin{\beta} - 2\cos{\alpha}\cos{\beta}} = \sqrt{2 - 2
\cos{ \left( \alpha - \beta \right)}}$$

Squaring both sides and subtracting 2, we find:
$$-2\sin{\alpha}\sin{\beta} - 2\cos{\alpha}\cos{\beta} = -2\cos{\left( \alpha -
\beta \right)}$$

Finally, we can divide both sides by negative 2 to get the difference of 
angles formula for cosine:
$$\cos{ \left( \alpha - \beta \right)} = \cos{\alpha}\cos{\beta} + \sin{\alpha}
\sin{\beta}$$

There are similar formulas for the sine and cosine of the sum of two angles, and
for the sine of the difference of two angles, which we won't derive here. 

\begin{mdframed}[style=important, frametitle={Sum and Difference Formulas}]
$$\cos{ \left( \alpha + \beta \right)} = \cos{\alpha}\cos{\beta} - \sin{\alpha}
\sin{\beta}$$
$$\cos{ \left( \alpha - \beta \right)} = \cos{\alpha}\cos{\beta} + \sin{\alpha}
\sin{\beta}$$
$$\sin{ \left( \alpha + \beta \right)} = \sin{\alpha}\cos{\beta} + \cos{\alpha}
\sin{\beta}$$
$$\sin{ \left( \alpha - \beta \right)} = \sin{\alpha}\cos{\beta} - \cos{\alpha}
\sin{\beta}$$
\end{mdframed}

\begin{Exercise}[label = sum_diff]
Without a calculator, find the exact value requested:
\begin{enumerate}
\item $\sin{\frac{\pi}{12}}$
\item $\cos{\frac{7\pi}{12}}$
\item $\tan{\frac{13\pi}{12}}$ (hint: $\tan{\theta} = \sin{\theta}/\cos{\theta}
$)
\end{enumerate}
\end{Exercise}

\begin{Answer}[ref = sum_diff]
\begin{enumerate}
\item $\sin{\left( \pi/12 \right) } = \sin{\left( \pi/3 - \pi/4 \right)} = 
\sin{\frac{\pi}{3}}\cos{\frac{\pi}{4}} - \cos{\frac{\pi}{3}}\sin{\frac{\pi}{4}}
= \left( \frac{\sqrt{3}}{2} \right) \cdot \left(  \frac{\sqrt{2}}{2} \right) - 
\left( \frac{1}{2} \right) \cdot \left( \frac{\sqrt{2}}{2} \right) = \frac{
\sqrt{6}}{4} - \frac{\sqrt{2}}{4} = \frac{\sqrt{6} - \sqrt{2}}{4}$
\item $\cos{\left( 7\pi/12 \right)} = \cos{\left( 4\pi/12 + 3\pi/12 \right)} = 
\cos{ \left( \pi/3 + \pi/4 \right)} = \cos{\frac{\pi}{3}}\cos{\frac{\pi}{4}} - 
\sin{\frac{\pi}{3}}\sin{\frac{\pi}{4}} = \left( \frac{1}{2} \right) \cdot 
\left( \frac{\sqrt{2}}{2} \right) - \left( \frac{\sqrt{3}}{2} \right) \cdot 
\left( \frac{\sqrt{2}}{2} \right) = \frac{\sqrt{2}}{4} - \frac{\sqrt{6}}{4} = 
\frac{\sqrt{2} - \sqrt{6}}{4}$
\item $\tan{ \left( 13\pi/12 \right)} = \frac{\sin{ \left( 13\pi/12 \right)}}{
\cos{ \left( 13\pi/12 \right)}}$ First, we will find $\sin{ \left( 13\pi/12 
\right)}$: $\sin{ \left( 13\pi/12 \right)} = \sin{\left( 3\pi/12 + 10\pi/12 
\right)} = \sin{\left( \pi/4 +  5\pi/6 \right)} = \sin{\frac{\pi}{4}}\cos{
\frac{5\pi}{6}} + \cos{\frac{\pi}{4}}\sin{\frac{5\pi}{6}} = \left( \frac{\sqrt{
2}}{2} \right) \cdot \left( \frac{-\sqrt{3}}{2} \right) + \left( \frac{\sqrt{2}
}{2} \right) \cdot \left( \frac{1}{2} \right) = \frac{-\sqrt{6}}{4} = \frac{
\sqrt{2}}{4} = \frac{\sqrt{2} - \sqrt{6}}{4}$. Next we find $\cos{\left( 13\pi/
12 \right)} = \cos{\left( \pi/4 + 5\pi/6 \right)} = \cos{\frac{\pi}{4}}\cos{
\frac{5\pi}{6}} - \sin{\frac{\pi}{4}}\sin{\frac{5\pi}{6}} = \left( \frac{\sqrt{
2}}{2} \right) \cdot \left( \frac{-\sqrt{3}}{2} \right) - \left( \frac{\sqrt{2
}}{2} \right) \cdot \left( \frac{1}{2} \right) = \frac{-\sqrt{6}}{4} - \frac{
\sqrt{2}}{4} = \frac{-\sqrt{6} - \sqrt{2}}{4}$. And therefore $\tan{ \left( 13
\pi/12 \right)} = \frac{\sin{13\pi/12}}{\cos{13\pi/12}} = \frac{\sqrt{2} - 
\sqrt{6}}{4} \cdot \frac{4}{-\sqrt{6} - \sqrt{2}} = \frac{\sqrt{6} - \sqrt{2}}{
\sqrt{6} + \sqrt{2}} = \frac{\sqrt{6} - \sqrt{2}}{\sqrt{6} + \sqrt{2}} \cdot 
\frac{\sqrt{6} - \sqrt{2}}{\sqrt{6} - \sqrt{2}} = \frac{6 - 2\sqrt{12} + 2}{6 -
2} = \frac{8 - 4\sqrt{3}}{4} = 2 - \sqrt{3}$ 
\end{enumerate}
\end{Answer}

\section{Double and Half Angle Formulas}
We can easily derive a formula for twice an angle by letting $\alpha = \beta$ 
for a sum formula. 

\textbf{Example}: Derive a formula for $\cos{2\theta}$ in terms of 
trigonometric functions of $\theta$.

\textbf{Solution}: Using the sum formula for cosine, we see that:
$$\cos{2\theta} = \cos{\left( \theta + \theta \right)}$$
$$= \cos{\theta}\cos{\theta} - \sin{\theta}\sin{\theta} = \cos^2{\theta} - 
\sin^2{\theta}$$
Noting that $\sin^2{\theta} = 1 - \cos^2{\theta}$:
\boxed{$$\cos{2\theta} = 2\cos^2{\theta} - 1$$}
Alternatively, we could note that $\cos^2{\theta} = 1 - \sin^2{\theta}$:
\boxed{$$\cos{2\theta} = 1 - 2\sin^2{\theta}$$}

Or additionally,
\boxed{$$\cos{2\theta} = \cos^2\theta - \sin^2\theta$$}


\begin{Exercise}[label = double_sine]
Derive a formula for $\sin{2\theta}$ in terms of trigonometric functions of 
$\theta$.
\vspace{50mm}
\end{Exercise}

\begin{Answer}[ref = double_sine]
$\sin{2\theta} = \sin{\theta + \theta} = \sin{\theta}\cos{\theta} + \cos{
\theta}\sin{\theta} = 2\sin{\theta}\cos{\theta}$
\end{Answer}

We can use these double-angle formulas for find half-angle formulas. Consider 
the double-angle formula for cosine:
$$\cos{2\theta} = 2\cos^2{\theta} - 1$$
Let $\theta = \alpha / 2$, then:
$$\cos{\alpha} = 2\cos^2{ \left( \alpha / 2 \right) } - 1$$
Rearranging to solve for $\cos{ \left( \alpha / 2 \right) }$:
$$2\cos^2{ \left( \alpha / 2 \right) } = \cos{\alpha} + 1$$
$$\cos^2{ \left( \alpha / 2 \right)} = \frac{\cos{\alpha} + 1}{2}$$
$$\cos{ \left( \alpha / 2 \right)} = \pm \sqrt{\frac{1 + \cos{\alpha}}{2}}$$

\begin{Exercise}[label = half_sine]
Derive a formula for $\sin{ \left( \alpha / 2 \right)}$.
\vspace{75mm}
\end{Exercise}

\begin{Answer}[ref = half_sine]
Similar to $\cos{ \left( \alpha / 2 \right)}$, we begin with the double angle 
formula for cosine, but another version:
$$\cos{2\theta} = 1 - 2\sin^2{\theta}$$
Substituting $\theta = \alpha / 2$:
$$\cos{\alpha} = 1 - 2\sin^2{ \left( \alpha / 2 \right)}$$
And rearranging to solve for $\sin{ \left( \alpha / 2 \right) }$:
$$\sin{ \left( \alpha / 2 \right) } = \pm \sqrt{\frac{1 - \cos{\alpha}}{2}}$$
\end{Answer}

There are two identities that will be very useful for integrals in a future 
chapter:
\begin{mdframed}[style=important, frametitle={Squared Trigonometric 
Identities}]
$$\sin^2{\theta} = \frac{1 - \cos{2\theta}}{2}$$
$$\cos^2{\theta} = \frac{1 + \cos{2\theta}}{2}$$
\end{mdframed}

These are just specific re-writings of the half-angle identities. 